Remove funcs and denote_funcs
At Adam's suggestion, we only need these for general recursion.
Removing them for now allows us to prototype code more quickly, since
our basic examples don't need general recusion.  We can instead use
[Fixpoint] to define recursive [Comp]utations.  (Although the rest of
the world may be attached to their non-termination, I'm definately
not.)

Computation.v
@@ -8,12 +8,10 @@ Reserved Notation "'call' f 'from' funcs [[ x ]]" (at level 35).
 
 Delimit Scope comp_scope with comp.
 
-Section funcs.
-  Variable funcs : string -> Type * Type.
+Section comp.
   Inductive Comp : Type -> Type :=
   | Return : forall A, A -> Comp A
   | Bind : forall A B, Comp A -> (A -> Comp B) -> Comp B
-  | Call : forall x, fst (funcs x) -> Comp (snd (funcs x))
   | Pick : forall A, Ensemble A -> Comp A.
 
   Bind Scope comp_scope with Comp.
@@ -32,9 +30,7 @@ Section funcs.
           then Return true
           else c2)%comp.
 
-  Section single_denote.
-    Variable denote_funcs : forall name, fst (funcs name) -> Comp (snd (funcs name)).
-
+  Section computes_to.
     Inductive computes_to
     : forall A : Type, Comp A -> A -> Prop :=
     | ReturnComputes : forall A v, @computes_to A (Return v) v
@@ -42,10 +38,7 @@ Section funcs.
                        @computes_to A comp_a comp_a_value
                        -> @computes_to B (f comp_a_value) comp_b_value
                        -> @computes_to B (Bind comp_a f) comp_b_value
-    | PickComputes : forall A (P : Ensemble A) v, P v -> @computes_to A (Pick P) v
-    | CallComputes : forall name (input : fst (funcs name)) (output_v : snd (funcs name)),
-                       @computes_to _ (denote_funcs name input) output_v
-                       -> @computes_to _ (Call name input) output_v.
+    | PickComputes : forall A (P : Ensemble A) v, P v -> @computes_to A (Pick P) v.
 
     Theorem computes_to_inv A (c : Comp A) v
     : computes_to c v -> match c with
@@ -53,19 +46,17 @@ Section funcs.
                            | Bind _ _ x f => fun v => exists comp_a_value,
                                                         computes_to x comp_a_value
                                                         /\ computes_to (f comp_a_value) v
-                           | Call name input => computes_to (denote_funcs name input)
                            | Pick _ P => P
                          end v.
     Proof.
       destruct 1; eauto.
     Qed.
+  End computes_to.
 
+  Section is_computational.
     (** A [Comp] is maximally computational if it could be written without [Pick] *)
     Inductive is_computational : forall A, Comp A -> Prop :=
     | Return_is_computational : forall A (x : A), is_computational (Return x)
-    | Call_is_computational : forall f x,
-                                is_computational (@denote_funcs f x)
-                                -> is_computational (@Call f x)
     | Bind_is_computational : forall A B (cA : Comp A) (f : A -> Comp B),
                                 is_computational cA
                                 -> (forall a,
@@ -79,64 +70,62 @@ Section funcs.
            | Bind _ _ x f => is_computational x
                              /\ forall v, computes_to x v
                                           -> is_computational (f v)
-           | Call name input => is_computational (denote_funcs name input)
            | Pick _ _ => False
          end.
     Proof.
       destruct 1; eauto.
     Qed.
+  End is_computational.
 
-    Section monad.
-      Local Ltac t :=
-        split;
-        intro;
-        repeat match goal with
-                 | [ H : _ |- _ ]
-                   => inversion H; clear H; subst; [];
-                      repeat match goal with
-                               | [ H : _ |- _ ] => apply inj_pair2 in H; subst
-                             end
-               end;
-        repeat first [ eassumption
-                     | solve [ constructor ]
-                     | eapply BindComputes; (eassumption || (try eassumption; [])) ].
+  Section monad.
+    Local Ltac t :=
+      split;
+      intro;
+      repeat match goal with
+               | [ H : _ |- _ ]
+                 => inversion H; clear H; subst; [];
+                    repeat match goal with
+                             | [ H : _ |- _ ] => apply inj_pair2 in H; subst
+                           end
+             end;
+      repeat first [ eassumption
+                   | solve [ constructor ]
+                   | eapply BindComputes; (eassumption || (try eassumption; [])) ].
 
-      Lemma bind_bind X Y Z (f : X -> Comp Y) (g : Y -> Comp Z) x v
-      : computes_to (Bind (Bind x f) g) v
-        <-> computes_to (Bind x (fun u => Bind (f u) g)) v.
-      Proof.
-        t.
-      Qed.
+    Lemma bind_bind X Y Z (f : X -> Comp Y) (g : Y -> Comp Z) x v
+    : computes_to (Bind (Bind x f) g) v
+      <-> computes_to (Bind x (fun u => Bind (f u) g)) v.
+    Proof.
+      t.
+    Qed.
 
-      Lemma bind_unit X Y (f : X -> Comp Y) x v
-      : computes_to (Bind (Return x) f) v
-        <-> computes_to (f x) v.
-      Proof.
-        t.
-      Qed.
+    Lemma bind_unit X Y (f : X -> Comp Y) x v
+    : computes_to (Bind (Return x) f) v
+      <-> computes_to (f x) v.
+    Proof.
+      t.
+    Qed.
 
-      Lemma unit_bind X (x : Comp X) v
-      : computes_to (Bind x (@Return X)) v
-        <-> computes_to x v.
-      Proof.
-        t.
-      Qed.
-    End monad.
-  End single_denote.
+    Lemma unit_bind X (x : Comp X) v
+    : computes_to (Bind x (@Return X)) v
+      <-> computes_to x v.
+    Proof.
+      t.
+    Qed.
+  End monad.
 
   (** The old program might be non-deterministic, and the new program
       less so.  This means we want to say that if [new] can compute to
       [v], then [old] should be able to compute to [v], too. *)
-  Definition refine old_denote_funcs new_denote_funcs {A} (old new : Comp A)
-    := forall v, computes_to new_denote_funcs new v
-                 -> computes_to old_denote_funcs old v.
+  Definition refine {A} (old new : Comp A)
+    := forall v, computes_to new v -> computes_to old v.
 
-  Global Instance refine_PreOrder denote_funcs A
-  : PreOrder (@refine denote_funcs denote_funcs A).
+  Global Instance refine_PreOrder A
+  : PreOrder (@refine A).
   Proof.
     split; compute in *; eauto.
   Qed.
-End funcs.
+End comp.
 
 Hint Constructors computes_to.
 
@@ -148,21 +137,20 @@ Ltac inversion_by rule :=
 Notation "x >>= y" := (Bind x y) : comp_scope.
 Notation "x <- y ; z" := (Bind y (fun x => z)) : comp_scope.
 Notation "x ;; z" := (Bind x (fun _ => z)) : comp_scope.
-Notation "'call' f 'from' funcs [[ x ]]" := (@Call funcs f x) : comp_scope.
-Notation "{ x  |  P }" := (@Pick _ _ (fun x => P)) : comp_scope.
-Notation "{ x : A  |  P }" := (@Pick _ A (fun x => P)) : comp_scope.
-Notation ret := (Return _).
+Notation "{ x  |  P }" := (@Pick _ (fun x => P)) : comp_scope.
+Notation "{ x : A  |  P }" := (@Pick A%type (fun x => P)) : comp_scope.
+Notation ret := Return.
 
-Add Parametric Relation funcs denote_funcs A : (Comp funcs A) (@refine funcs denote_funcs denote_funcs A)
+Add Parametric Relation A : (Comp A) (@refine A)
   reflexivity proved by reflexivity
   transitivity proved by transitivity
     as refine_rel.
 
-Add Parametric Morphism funcs denote_funcs A B : (@Bind funcs A B)
+Add Parametric Morphism A B : (@Bind A B)
   with signature
-  (@refine funcs denote_funcs denote_funcs A)
-    ==> (pointwise_relation _ (@refine funcs denote_funcs denote_funcs B))
-    ==> (@refine funcs denote_funcs denote_funcs B)
+  (@refine A)
+    ==> (pointwise_relation _ (@refine B))
+    ==> (@refine B)
     as refine_bind.
 Proof.
   intros.
@@ -173,11 +161,8 @@ Proof.
 Qed.
 
 Section general_refine_lemmas.
-  Variable funcs : string -> Type * Type.
-
-  Lemma refine_pick_pair denote_funcs A B (PA : A -> Prop) (PB : B -> Prop)
-  : refine (funcs := funcs) denote_funcs denote_funcs
-           { x : A * B | PA (fst x) /\ PB (snd x) }%comp
+  Lemma refine_pick_pair A B (PA : A -> Prop) (PB : B -> Prop)
+  : refine { x : A * B | PA (fst x) /\ PB (snd x) }%comp
            (a <- { a : A | PA a };
             b <- { b : B | PB b };
             ret (a, b))%comp.
