ADTImplementation.v
@@ -42,58 +42,51 @@ Ltac generic_impl_t ADTimpl MutatorMethodSpecs ObserverMethodsCorrect MutatorMet
 
 (** * Basic ADT definitions *)
 Section comp_env.
-  (** We have one ambiant [funcs] around for everything. *)
-  Variable funcs : string -> Type * Type.
-
   (** One implementation of an ADT *)
-  Record ADTimpl
-         (denote_funcs : forall name, fst (funcs name) -> Comp funcs (snd (funcs name)))
-         (A : ADT)
-    :=
-      {
-        State : Type;
-        (** Real state type in Gallina *)
+  Record ADTimpl (A : ADT) :=
+    {
+      State : Type;
+      (** Real state type in Gallina *)
 
-        RepInv : Model A -> State -> Prop;
-        (** Relationship between abstract (specification) and concrete (implementation) states *)
+      RepInv : Model A -> State -> Prop;
+      (** Relationship between abstract (specification) and concrete (implementation) states *)
 
-        MutatorMethodBodies : MutatorIndex A -> methodTypeD funcs State;
-        (** An implementation of each mutator method *)
+      MutatorMethodBodies : MutatorIndex A -> methodTypeD State;
+      (** An implementation of each mutator method *)
 
-        ObserverMethodBodies : ObserverIndex A -> methodTypeD funcs State;
-        (** An implementation of each observer method *)
+      ObserverMethodBodies : ObserverIndex A -> methodTypeD State;
+      (** An implementation of each observer method *)
 
-        MutatorMethodsCorrect : forall idx, mutatorMethodCorrect
-                                              denote_funcs
-                                              (MutatorMethodSpecs A idx)
-                                              RepInv
-                                              (MutatorMethodBodies idx);
-        (** All mutator methods satisfy their specs. *)
+      MutatorMethodsCorrect : forall idx, mutatorMethodCorrect
 
-        ObserverMethodsCorrect : forall idx, observerMethodCorrect
-                                               denote_funcs
-                                               (ObserverMethodSpecs A idx)
-                                               RepInv
-                                               (ObserverMethodBodies idx)
-      (** All observer methods satisfy their specs. *)
-      }.
+                                            (MutatorMethodSpecs A idx)
+                                            RepInv
+                                            (MutatorMethodBodies idx);
+      (** All mutator methods satisfy their specs. *)
 
-  Definition ADTimpl_is_computational denote_funcs A (Ai : ADTimpl denote_funcs A) : Prop
+      ObserverMethodsCorrect : forall idx, observerMethodCorrect
+
+                                             (ObserverMethodSpecs A idx)
+                                             RepInv
+                                             (ObserverMethodBodies idx)
+    (** All observer methods satisfy their specs. *)
+    }.
+
+  Definition ADTimpl_is_computational A (Ai : ADTimpl A) : Prop
     := (forall i s x,
           (exists m, RepInv Ai m s)
-          -> is_computational denote_funcs (MutatorMethodBodies Ai i s x))
+          -> is_computational (MutatorMethodBodies Ai i s x))
        /\ (forall i s x,
              (exists m, RepInv Ai m s)
-             -> is_computational denote_funcs (ObserverMethodBodies Ai i s x)).
+             -> is_computational (ObserverMethodBodies Ai i s x)).
 
-  Ltac impl_t'' denote_funcs := generic_impl_t'' (@ADTimpl denote_funcs) MutatorMethodSpecs (@ObserverMethodsCorrect denote_funcs) (@MutatorMethodsCorrect denote_funcs).
-  Ltac impl_t' denote_funcs := generic_impl_t' (@ADTimpl denote_funcs) MutatorMethodSpecs (@ObserverMethodsCorrect denote_funcs) (@MutatorMethodsCorrect denote_funcs).
-  Ltac impl_t denote_funcs := generic_impl_t (@ADTimpl denote_funcs) MutatorMethodSpecs (@ObserverMethodsCorrect denote_funcs) (@MutatorMethodsCorrect denote_funcs).
+  Ltac impl_t'' := generic_impl_t'' (@ADTimpl) MutatorMethodSpecs (@ObserverMethodsCorrect) (@MutatorMethodsCorrect).
+  Ltac impl_t' := generic_impl_t' (@ADTimpl) MutatorMethodSpecs (@ObserverMethodsCorrect) (@MutatorMethodsCorrect).
+  Ltac impl_t := generic_impl_t (@ADTimpl) MutatorMethodSpecs (@ObserverMethodsCorrect) (@MutatorMethodsCorrect).
 
   (** * A simple pairing combinator *)
 
   Section paired.
-    Variable denote_funcs : forall name, fst (funcs name) -> Comp funcs (snd (funcs name)).
     Variables A B : ADT.
     (** Let's compose these two ADTs. *)
 
@@ -120,10 +113,10 @@ Section comp_env.
       |}.
 
     (** Now we show how to implement it. *)
-    Variable Ai : ADTimpl denote_funcs A.
-    Variable Bi : ADTimpl denote_funcs B.
+    Variable Ai : ADTimpl A.
+    Variable Bi : ADTimpl B.
 
-    Definition pairedImpl : ADTimpl denote_funcs pairedADT.
+    Definition pairedImpl : ADTimpl pairedADT.
     Proof.
       refine {|
           State := State Ai * State Bi;
@@ -148,12 +141,11 @@ Section comp_env.
                        ret ((fst s, fst sy'), snd sy'))%comp
                end
         |};
-      abstract impl_t denote_funcs idtac.
+      abstract impl_t idtac.
     Defined.
   End paired.
 
   Section prod.
-    Variable denote_funcs : forall name, fst (funcs name) -> Comp funcs (snd (funcs name)).
     Variable model : Type.
     Variables AMutIndex BMutIndex AObsIndex BObsIndex : Type.
     Variable AMutSpec : AMutIndex -> mutatorMethodSpec model.
@@ -189,8 +181,8 @@ Section comp_env.
       |}.
 
     (** Now we show how to implement it. *)
-    Variable Ai : ADTimpl denote_funcs A.
-    Variable Bi : ADTimpl denote_funcs B.
+    Variable Ai : ADTimpl A.
+    Variable Bi : ADTimpl B.
 
     (*Local Hint Extern 1 (@ex (_ * _) _) => eexists (_, _).*)
 
@@ -203,7 +195,7 @@ Section comp_env.
 
     Local Hint Extern 1 => apply symmetry.
 
-    Definition prodImpl : ADTimpl denote_funcs prodADT.
+    Definition prodImpl : ADTimpl prodADT.
       refine {|
           State := State Ai * State Bi;
           RepInv := fun (m : Model prodADT) s
@@ -229,12 +221,12 @@ Section comp_env.
       abstract (
           intro idx;
           try (assert (MM := mutators_match idx));
-          impl_t' denote_funcs idtac;
+          impl_t' idtac;
           match goal with
             | [ AM : AMutSpec _ _ _ _, BM : BMutSpec _ _ _ _ |- _ ]
               => specialize (MM _ _ _ _ AM BM); subst
           end;
-          impl_t denote_funcs idtac
+          impl_t idtac
         ).
     Defined.
   End prod.
@@ -242,8 +234,6 @@ Section comp_env.
   (** A transformation (approximately, injection) from one ADT to another *)
 
   Section inj.
-    Variable denote_funcs : forall name, fst (funcs name) -> Comp funcs (snd (funcs name)).
-
     Variables A B : ADT.
     (** Let's compose these two ADTs. *)
 
@@ -261,9 +251,9 @@ Section comp_env.
         ObserverMethodSpecs A (observerMap idx) (BtoA m) x y
         -> ObserverMethodSpecs B idx m x y.
 
-    Variable Ai : ADTimpl denote_funcs A.
+    Variable Ai : ADTimpl A.
 
-    Definition injImpl : ADTimpl denote_funcs B.
+    Definition injImpl : ADTimpl B.
     Proof.
       refine {|
           State := State Ai;
@@ -273,9 +263,9 @@ Section comp_env.
           ObserverMethodBodies name := ObserverMethodBodies Ai (observerMap name)
         |};
       abstract (
-          impl_t' denote_funcs idtac;
+          impl_t' idtac;
           edestruct mutatorSpecMap; try eassumption;
-          impl_t denote_funcs idtac
+          impl_t idtac
         ).
     Defined.
   End inj.
@@ -283,13 +273,11 @@ Section comp_env.
 
   (** Every spec is trivially implementable using [Pick]. *)
   Section pick.
-    Variable denote_funcs : forall name, fst (funcs name) -> Comp funcs (snd (funcs name)).
-
     Variables A : ADT.
     Variable state : Type.
     Variable rep_inv : Model A -> state -> Prop.
 
-    Definition pickImpl : ADTimpl denote_funcs A.
+    Definition pickImpl : ADTimpl A.
     Proof.
       refine {|
           State := state;
@@ -328,27 +316,22 @@ Section comp_env.
   (** We can [refine] the computations of an implementation *)
 
   Section inj_by_refine.
-    Variables old_denote_funcs new_denote_funcs
-    : forall name, fst (funcs name) -> Comp funcs (snd (funcs name)).
-
     Variable A : ADT.
-    Variable Ai : ADTimpl old_denote_funcs A.
+    Variable Ai : ADTimpl A.
 
-    Variable new_mutators : MutatorIndex A -> methodTypeD funcs (State Ai).
-    Variable new_observers : ObserverIndex A -> methodTypeD funcs (State Ai).
+    Variable new_mutators : MutatorIndex A -> methodTypeD (State Ai).
+    Variable new_observers : ObserverIndex A -> methodTypeD (State Ai).
 
     Hypothesis mutator_refinement
     : forall idx s x,
-        refine old_denote_funcs new_denote_funcs
-               (MutatorMethodBodies Ai idx s x)
+        refine (MutatorMethodBodies Ai idx s x)
                (new_mutators idx s x).
     Hypothesis observer_refinement
     : forall idx s x,
-        refine old_denote_funcs new_denote_funcs
-               (ObserverMethodBodies Ai idx s x)
+        refine (ObserverMethodBodies Ai idx s x)
                (new_observers idx s x).
 
-    Definition inj_refine_Impl : ADTimpl new_denote_funcs A.
+    Definition inj_refine_Impl : ADTimpl A.
     Proof.
       refine {|
           State := State Ai;
@@ -356,7 +339,7 @@ Section comp_env.
           MutatorMethodBodies := new_mutators;
           ObserverMethodBodies := new_observers
         |};
-      abstract impl_t old_denote_funcs ltac:(eapply mutator_refinement).
+      abstract impl_t ltac:(eapply mutator_refinement).
     Defined.
   End inj_by_refine.
 End comp_env.
